% Equation 1
\begin{dmath}
0={{\sigma}}\, {{\hat {\bar c}}}_{t}+{{\varphi}}\, {{\hat {\bar y}}}_{t}+{{\alpha}}\, {{\bar s}}_{t}-\left(1+{{\varphi}}\right)\, {{a}}_{t}
\end{dmath}
% Equation 2
\begin{dmath}
0={{\sigma}}\, {{\hat {\bar c}^*}}_{t}+{{\varphi}}\, {{\hat {\bar y}^*}}_{t}-{{\bar s}}_{t}\, {{\alpha^*}}-\left(1+{{\varphi}}\right)\, {{a^*}}_{t}
\end{dmath}
% Equation 3
\begin{dmath}
{{\tilde{\sigma}}}\, \left({{\hat {\bar y}}}_{t}-{{\delta}}\, {{\hat {\bar g}}}_{t}\right)={{\sigma}}\, {{\hat {\bar c}}}_{t}+{{\bar s}}_{t}\, {{\bar{\alpha}}}\, \left(1-{{h}}\right)\, {{w_{\bar{\alpha}}}}
\end{dmath}
% Equation 4
\begin{dmath}
{{\tilde{\sigma}}}\, \left({{\hat {\bar y}^*}}_{t}-{{\delta}}\, {{\hat {\bar g}^*}}_{t}\right)={{\sigma}}\, {{\hat {\bar c}^*}}_{t}-{{\bar s}}_{t}\, {{w_{\bar{\alpha}}}}\, {{\bar{\alpha}}}\, {{h}}
\end{dmath}
% Equation 5
\begin{dmath}
{{\bar s}}_{t}={{\tilde\sigma_{\bar{\alpha}}}}\, \left({{\hat {\bar y}}}_{t}-{{\hat {\bar y}^*}}_{t}-{{\delta}}\, \left({{\hat {\bar g}}}_{t}-{{\hat {\bar g}^*}}_{t}\right)\right)
\end{dmath}
% Equation 6
\begin{dmath}
{{\hat {\bar g}}}_{t}\, {{\gamma}}={{\sigma}}\, {{\hat {\bar c}}}_{t}+{{\alpha}}\, {{\bar s}}_{t}
\end{dmath}
% Equation 7
\begin{dmath}
{{\hat {\bar g}^*}}_{t}\, {{\gamma}}={{\sigma}}\, {{\hat {\bar c}^*}}_{t}-{{\bar s}}_{t}\, {{\alpha^*}}
\end{dmath}
% Equation 8
\begin{dmath}
{{\bar s^*}}_{t}=\left(-{{\bar s}}_{t}\right)
\end{dmath}
% Equation 9
\begin{dmath}
{{\hat {\bar c}^H}}_{t}={{\hat {\bar c}}}_{t}+{{\bar s}}_{t}\, {{\alpha}}\, {{\eta}}
\end{dmath}
% Equation 10
\begin{dmath}
{{\hat {\bar c}^F}}_{t}={{\hat {\bar c}}}_{t}+{{\bar s}}_{t}\, \left(-{{\eta}}\right)\, \left(1-{{\alpha}}\right)
\end{dmath}
% Equation 11
\begin{dmath}
{{\hat {\bar c}^{H*}}}_{t}={{\hat {\bar c}^*}}_{t}+{{\bar s}}_{t}\, {{\eta}}\, \left(1-{{\alpha^*}}\right)
\end{dmath}
% Equation 12
\begin{dmath}
{{\hat {\bar c}^{F*}}}_{t}={{\hat {\bar c}^*}}_{t}+{{\bar s}}_{t}\, {{\alpha^*}}\, \left(-{{\eta}}\right)
\end{dmath}
% Equation 13
\begin{dmath}
{{\hat {\bar n}}}_{t}={{\hat {\bar y}}}_{t}-{{a}}_{t}
\end{dmath}
% Equation 14
\begin{dmath}
{{\hat {\bar n}^*}}_{t}={{\hat {\bar y}^*}}_{t}-{{a^*}}_{t}
\end{dmath}
% Equation 15
\begin{dmath}
{{\hat {\bar f}}}_{t}={{\hat {\bar g}}}_{t}-{{\hat {\bar y}}}_{t}
\end{dmath}
% Equation 16
\begin{dmath}
{{\hat {\bar f}^*}}_{t}={{\hat {\bar g}^*}}_{t}-{{\hat {\bar y}^*}}_{t}
\end{dmath}
% Equation 17
\begin{dmath}
{{\bar r}}_{t}=\left(1+{{\varphi}}\right)\, \left({{a}}_{t+1}-{{a}}_{t}\right)-{{\varphi}}\, \left({{\hat {\bar y}}}_{t+1}-{{\hat {\bar y}}}_{t}\right)
\end{dmath}
% Equation 18
\begin{dmath}
{{\bar r^*}}_{t}=\left(1+{{\varphi}}\right)\, \left({{a^*}}_{t+1}-{{a^*}}_{t}\right)-{{\varphi}}\, \left({{\hat {\bar y}^*}}_{t+1}-{{\hat {\bar y}^*}}_{t}\right)
\end{dmath}
% Equation 19
\begin{dmath}
{{\hat {\bar y}^{cu}}}_{t}={{\hat {\bar y}}}_{t}\, {{h}}+{{\hat {\bar y}^*}}_{t}\, \left(1-{{h}}\right)
\end{dmath}
% Equation 20
\begin{dmath}
{{\hat {\bar g}^{cu}}}_{t}={{\hat {\bar g}}}_{t}\, {{h}}+\left(1-{{h}}\right)\, {{\hat {\bar g}^*}}_{t}
\end{dmath}
% Equation 21
\begin{dmath}
{{\hat {\bar c}^{cu}}}_{t}={{\hat {\bar c}}}_{t}\, {{h}}+{{\hat {\bar c}^*}}_{t}\, \left(1-{{h}}\right)
\end{dmath}
% Equation 22
\begin{dmath}
{{\hat {\bar r}^{cu}}}_{t}={{h}}\, {{\bar r}}_{t}+\left(1-{{h}}\right)\, {{\bar r^*}}_{t}
\end{dmath}
% Equation 23
\begin{dmath}
{{\hat {\bar c}^{H,cu}}}_{t}={{h}}\, {{\hat {\bar c}^H}}_{t}+\left(1-{{h}}\right)\, {{\hat {\bar c}^{H*}}}_{t}
\end{dmath}
% Equation 24
\begin{dmath}
{{\hat {\bar c}^{F,cu}}}_{t}={{h}}\, {{\hat {\bar c}^F}}_{t}+\left(1-{{h}}\right)\, {{\hat {\bar c}^{F*}}}_{t}
\end{dmath}
% Equation 25
\begin{dmath}
{{\hat {\bar f}^{H,cu}}}_{t}={{h}}\, {{\hat {\bar f}}}_{t}+\left(1-{{h}}\right)\, {{\hat {\bar f}^*}}_{t}
\end{dmath}
% Equation 26
\begin{dmath}
{{\hat {\bar n}^{H,cu}}}_{t}={{h}}\, {{\hat {\bar n}}}_{t}+\left(1-{{h}}\right)\, {{\hat {\bar n}^*}}_{t}
\end{dmath}
% Equation 27
\begin{dmath}
{{\bar{nx}}}_{t}={{\hat {\bar y}}}_{t}-\left(1-{{\delta}}\right)\, \left({{\hat {\bar c}}}_{t}+{{\alpha}}\, {{\bar s}}_{t}\right)-{{\delta}}\, {{\hat {\bar g}}}_{t}
\end{dmath}
% Equation 28
\begin{dmath}
{{\bar{nx}^*}}_{t}={{\hat {\bar y}^*}}_{t}-\left(1-{{\delta}}\right)\, \left({{\hat {\bar c}^*}}_{t}+{{\alpha^*}}\, {{\bar s^*}}_{t}\right)-{{\delta}}\, {{\hat {\bar g}^*}}_{t}
\end{dmath}
% Equation 29
\begin{dmath}
{{\hat {\bar{nx}}^{H,cu}}}_{t}={{h}}\, {{\bar{nx}}}_{t}+\left(1-{{h}}\right)\, {{\bar{nx}^*}}_{t}
\end{dmath}
% Equation 30
\begin{dmath}
{{\pi^H}}_{t}={{\beta}}\, {{\pi^H}}_{t+1}+{{\lambda}}\, \left(\left({{\varphi}}+{{\tilde\sigma_{\bar{\alpha}}}}\, {{\Omega_{\bar \alpha,h}}}\right)\, {{\hat y}}_{t}-{{\delta}}\, {{\tilde\sigma_{\bar{\alpha}}}}\, {{\Omega_{\bar \alpha,h}}}\, {{\hat g}}_{t}+\left({{\tilde{\sigma}}}-{{\tilde\sigma_{\bar{\alpha}}}}\, {{\Omega_{\bar \alpha,h}}}\right)\, \left({{\hat y^*}}_{t}-{{\delta}}\, {{\hat g^*}}_{t}\right)-\left(1+{{\varphi}}\right)\, {{a}}_{t}\right)
\end{dmath}
% Equation 31
\begin{dmath}
{{\pi^{F*}}}_{t}={{\beta}}\, {{\pi^{F*}}}_{t+1}+{{\lambda^*}}\, \left({{\hat y^*}}_{t}\, \left({{\varphi}}+{{\tilde\sigma_{\bar{\alpha}}}}\, {{\Omega_{\bar \alpha,1-h}}}\right)-{{\hat g^*}}_{t}\, {{\delta}}\, {{\tilde\sigma_{\bar{\alpha}}}}\, {{\Omega_{\bar \alpha,1-h}}}+\left({{\tilde{\sigma}}}-{{\tilde\sigma_{\bar{\alpha}}}}\, {{\Omega_{\bar \alpha,1-h}}}\right)\, \left({{\hat y}}_{t}-{{\delta}}\, {{\hat g}}_{t}\right)-\left(1+{{\varphi}}\right)\, {{a^*}}_{t}\right)
\end{dmath}
% Equation 32
\begin{dmath}
{{\hat y}}_{t}={{\hat y}}_{t+1}-{{\delta}}\, \left({{\hat g}}_{t+1}-{{\hat g}}_{t}\right)-\frac{1}{{{\tilde\sigma_{\bar{\alpha}}}}\, {{\Omega_{\bar \alpha,h}}}}\, \left({{i}}_{t}-{{\pi^H}}_{t+1}\right)+\left(\frac{1+{{\bar{\alpha}}}\, {{\Theta{\bar{\alpha}}}}}{{{\Omega_{\bar \alpha,h}}}}-1\right)\, \left({{\hat y^*}}_{t+1}-{{\hat y^*}}_{t}-{{\delta}}\, \left({{\hat g^*}}_{t+1}-{{\hat g^*}}_{t}\right)\right)
\end{dmath}
% Equation 33
\begin{dmath}
{{\hat y^*}}_{t}={{\hat y^*}}_{t+1}-{{\delta}}\, \left({{\hat g^*}}_{t+1}-{{\hat g^*}}_{t}\right)-\frac{1}{{{\tilde\sigma_{\bar{\alpha}}}}\, {{\Omega_{\bar \alpha,1-h}}}}\, \left({{i^*}}_{t}-{{\pi^{F*}}}_{t+1}\right)+\left(\frac{1+{{\bar{\alpha}}}\, {{\Theta{\bar{\alpha}}}}}{{{\Omega_{\bar \alpha,1-h}}}}-1\right)\, \left({{\hat y}}_{t+1}-{{\hat y}}_{t}-{{\delta}}\, \left({{\hat g}}_{t+1}-{{\hat g}}_{t}\right)\right)
\end{dmath}
% Equation 34
\begin{dmath}
{{s}}_{t}={{\tilde\sigma_{\bar{\alpha}}}}\, \left({{\hat y}}_{t}-{{\hat y^*}}_{t}-{{\delta}}\, \left({{\hat g}}_{t}-{{\hat g^*}}_{t}\right)\right)
\end{dmath}
% Equation 35
\begin{dmath}
{{s^*}}_{t}=\left(-{{s}}_{t}\right)
\end{dmath}
% Equation 36
\begin{dmath}
{{\hat n}}_{t}={{\hat y}}_{t}-{{a}}_{t}
\end{dmath}
% Equation 37
\begin{dmath}
{{\hat n^*}}_{t}={{\hat y^*}}_{t}-{{a^*}}_{t}
\end{dmath}
% Equation 38
\begin{dmath}
{{\tilde{\sigma}}}\, \left({{\hat y}}_{t}-{{\delta}}\, {{\hat g}}_{t}\right)={{\sigma}}\, {{\hat c}}_{t}+{{\bar{\alpha}}}\, \left(1-{{h}}\right)\, {{w_{\bar{\alpha}}}}\, {{s}}_{t}
\end{dmath}
% Equation 39
\begin{dmath}
{{\tilde{\sigma}}}\, \left({{\hat y^*}}_{t}-{{\delta}}\, {{\hat g^*}}_{t}\right)={{\sigma}}\, {{\hat c^*}}_{t}-{{w_{\bar{\alpha}}}}\, {{\bar{\alpha}}}\, {{h}}\, {{s}}_{t}
\end{dmath}
% Equation 40
\begin{dmath}
{{\hat f}}_{t}={{\hat g}}_{t}-{{\hat y}}_{t}
\end{dmath}
% Equation 41
\begin{dmath}
{{\hat f^*}}_{t}={{\hat g^*}}_{t}-{{\hat y^*}}_{t}
\end{dmath}
% Equation 42
\begin{dmath}
{{\hat c^H}}_{t}={{\hat c}}_{t}+{{\alpha}}\, {{\eta}}\, {{s}}_{t}
\end{dmath}
% Equation 43
\begin{dmath}
{{\hat c^F}}_{t}={{\hat c}}_{t}+\left(-{{\eta}}\right)\, \left(1-{{\alpha}}\right)\, {{s}}_{t}
\end{dmath}
% Equation 44
\begin{dmath}
{{\hat c^{H*}}}_{t}={{\hat c^*}}_{t}+{{\eta}}\, \left(1-{{\alpha^*}}\right)\, {{s}}_{t}
\end{dmath}
% Equation 45
\begin{dmath}
{{\hat c^{F*}}}_{t}={{\hat c^*}}_{t}+{{\alpha^*}}\, \left(-{{\eta}}\right)\, {{s}}_{t}
\end{dmath}
% Equation 46
\begin{dmath}
{{i}}_{t}={{i^{cu}}}_{t}
\end{dmath}
% Equation 47
\begin{dmath}
{{i^*}}_{t}={{i^{cu}}}_{t}
\end{dmath}
% Equation 48
\begin{dmath}
{{\pi^{cu}}}_{t}={{h}}\, {{\pi^H}}_{t}+\left(1-{{h}}\right)\, {{\pi^{F*}}}_{t}
\end{dmath}
% Equation 49
\begin{dmath}
{{\hat y^{cu}}}_{t}={{h}}\, {{\hat y}}_{t}+\left(1-{{h}}\right)\, {{\hat y^*}}_{t}
\end{dmath}
% Equation 50
\begin{dmath}
{{\hat g^{cu}}}_{t}={{h}}\, {{\hat g}}_{t}+\left(1-{{h}}\right)\, {{\hat g^*}}_{t}
\end{dmath}
% Equation 51
\begin{dmath}
{{\hat c^{cu}}}_{t}={{h}}\, {{\hat c}}_{t}+\left(1-{{h}}\right)\, {{\hat c^*}}_{t}
\end{dmath}
% Equation 52
\begin{dmath}
{{\hat c^{H,cu}}}_{t}={{h}}\, {{\hat c^H}}_{t}+\left(1-{{h}}\right)\, {{\hat c^{H*}}}_{t}
\end{dmath}
% Equation 53
\begin{dmath}
{{\hat c^{F,cu}}}_{t}={{h}}\, {{\hat c^F}}_{t}+\left(1-{{h}}\right)\, {{\hat c^{F*}}}_{t}
\end{dmath}
% Equation 54
\begin{dmath}
{{\hat f^{cu}}}_{t}={{h}}\, {{\hat f}}_{t}+\left(1-{{h}}\right)\, {{\hat f^*}}_{t}
\end{dmath}
% Equation 55
\begin{dmath}
{{\hat n^{cu}}}_{t}={{h}}\, {{\hat n}}_{t}+\left(1-{{h}}\right)\, {{\hat n^*}}_{t}
\end{dmath}
% Equation 56
\begin{dmath}
{{nx}}_{t}={{\hat y}}_{t}-\left(1-{{\delta}}\right)\, \left({{\hat c}}_{t}+{{\alpha}}\, {{s}}_{t}\right)-{{\delta}}\, {{\hat g}}_{t}
\end{dmath}
% Equation 57
\begin{dmath}
{{nx^*}}_{t}={{\hat y^*}}_{t}-\left(1-{{\delta}}\right)\, \left({{\hat c^*}}_{t}+{{\alpha^*}}\, {{s^*}}_{t}\right)-{{\delta}}\, {{\hat g^*}}_{t}
\end{dmath}
% Equation 58
\begin{dmath}
{{\hat{nx}^{cu}}}_{t}={{h}}\, {{nx}}_{t}+\left(1-{{h}}\right)\, {{nx^*}}_{t}
\end{dmath}
% Equation 59
\begin{dmath}
{{\tilde y}}_{t}={{\hat y}}_{t}-{{\hat {\bar y}}}_{t}
\end{dmath}
% Equation 60
\begin{dmath}
{{\tilde g}}_{t}={{\hat g}}_{t}-{{\hat {\bar g}}}_{t}
\end{dmath}
% Equation 61
\begin{dmath}
{{\tilde c}}_{t}={{\hat c}}_{t}-{{\hat {\bar c}}}_{t}
\end{dmath}
% Equation 62
\begin{dmath}
{{\tilde c^H}}_{t}={{\hat c^H}}_{t}-{{\hat {\bar c}^H}}_{t}
\end{dmath}
% Equation 63
\begin{dmath}
{{\tilde c^F}}_{t}={{\hat c^F}}_{t}-{{\hat {\bar c}^F}}_{t}
\end{dmath}
% Equation 64
\begin{dmath}
{{\tilde n}}_{t}={{\hat n}}_{t}-{{\hat {\bar n}}}_{t}
\end{dmath}
% Equation 65
\begin{dmath}
{{\tilde f}}_{t}={{\hat f}}_{t}-{{\hat {\bar f}}}_{t}
\end{dmath}
% Equation 66
\begin{dmath}
{{\tilde s}}_{t}={{s}}_{t}-{{\bar s}}_{t}
\end{dmath}
% Equation 67
\begin{dmath}
{{\tilde i}}_{t}={{i}}_{t}-{{\bar r}}_{t}
\end{dmath}
% Equation 68
\begin{dmath}
{{\tilde y^*}}_{t}={{\hat y^*}}_{t}-{{\hat {\bar y}^*}}_{t}
\end{dmath}
% Equation 69
\begin{dmath}
{{\tilde g^*}}_{t}={{\hat g^*}}_{t}-{{\hat {\bar g}^*}}_{t}
\end{dmath}
% Equation 70
\begin{dmath}
{{\tilde c^*}}_{t}={{\hat c^*}}_{t}-{{\hat {\bar c}^*}}_{t}
\end{dmath}
% Equation 71
\begin{dmath}
{{\tilde c^{H*}}}_{t}={{\hat c^{H*}}}_{t}-{{\hat {\bar c}^{H*}}}_{t}
\end{dmath}
% Equation 72
\begin{dmath}
{{\tilde c^{F*}}}_{t}={{\hat c^{F*}}}_{t}-{{\hat {\bar c}^{F*}}}_{t}
\end{dmath}
% Equation 73
\begin{dmath}
{{\tilde n^*}}_{t}={{\hat n^*}}_{t}-{{\hat {\bar n}^*}}_{t}
\end{dmath}
% Equation 74
\begin{dmath}
{{\tilde f^*}}_{t}={{\hat f^*}}_{t}-{{\hat {\bar f}^*}}_{t}
\end{dmath}
% Equation 75
\begin{dmath}
{{\tilde s^*}}_{t}={{s^*}}_{t}-{{\bar s^*}}_{t}
\end{dmath}
% Equation 76
\begin{dmath}
{{\tilde i^*}}_{t}={{i^*}}_{t}-{{\bar r^*}}_{t}
\end{dmath}
% Equation 77
\begin{dmath}
{{\tilde y^{cu}}}_{t}={{h}}\, {{\tilde y}}_{t}+\left(1-{{h}}\right)\, {{\tilde y^*}}_{t}
\end{dmath}
% Equation 78
\begin{dmath}
{{\tilde g^{cu}}}_{t}={{h}}\, {{\tilde g}}_{t}+\left(1-{{h}}\right)\, {{\tilde g^*}}_{t}
\end{dmath}
% Equation 79
\begin{dmath}
{{\tilde c^{cu}}}_{t}={{h}}\, {{\tilde c}}_{t}+\left(1-{{h}}\right)\, {{\tilde c^*}}_{t}
\end{dmath}
% Equation 80
\begin{dmath}
{{\tilde i^{cu}}}_{t}={{i}}_{t}-{{\hat {\bar r}^{cu}}}_{t}
\end{dmath}
% Equation 81
\begin{dmath}
{{\tilde g^{r}}}_{t}={{\tilde g}}_{t}-{{\tilde g^*}}_{t}
\end{dmath}
% Equation 82
\begin{dmath}
{{\tilde n^{cu}}}_{t}={{\hat n^{cu}}}_{t}-{{\hat {\bar n}^{H,cu}}}_{t}
\end{dmath}
% Equation 83
\begin{dmath}
{{\tilde f^{cu}}}_{t}={{h}}\, {{\tilde f}}_{t}+\left(1-{{h}}\right)\, {{\tilde f^*}}_{t}
\end{dmath}
% Equation 84
\begin{dmath}
{{\tilde c^{H,cu}}}_{t}={{h}}\, {{\tilde c^H}}_{t}+\left(1-{{h}}\right)\, {{\tilde c^{H*}}}_{t}
\end{dmath}
% Equation 85
\begin{dmath}
{{\tilde c^{F,cu}}}_{t}={{h}}\, {{\tilde c^F}}_{t}+\left(1-{{h}}\right)\, {{\tilde c^{F*}}}_{t}
\end{dmath}
% Equation 86
\begin{dmath}
{{\tilde{nx}}}_{t}={{nx}}_{t}-{{\bar{nx}}}_{t}
\end{dmath}
% Equation 87
\begin{dmath}
{{\tilde{nx}^*}}_{t}={{nx^*}}_{t}-{{\bar{nx}^*}}_{t}
\end{dmath}
% Equation 88
\begin{dmath}
{{\tilde{nx}^{cu}}}_{t}={{h}}\, {{\tilde{nx}}}_{t}+\left(1-{{h}}\right)\, {{\tilde{nx}^*}}_{t}
\end{dmath}
% Equation 89
\begin{dmath}
{{i^{cu}}}_{t}-{{\hat {\bar r}^{cu}}}_{t}=0.7\, \left({{i^{cu}}}_{t-1}-{{\hat {\bar r}^{cu}}}_{t-1}\right)+{{\pi^{cu}}}_{t}\, 2.5+{{\tilde y^{cu}}}_{t}\, 0.125
\end{dmath}
% Equation 90
\begin{dmath}
{{\tilde g}}_{t}={RHOG}\, {{\tilde g}}_{t-1}+{FP\_y\_gapH}\, \left({{\tilde y}}_{t-1}-{{\tilde y^{cu}}}_{t-1}\right)+{FP\_pieH}\, \left({{\pi^H}}_{t-1}-{{\pi^{cu}}}_{t-1}\right)
\end{dmath}
% Equation 91
\begin{dmath}
{{\tilde g^*}}_{t}={RHOG}\, {{\tilde g^*}}_{t-1}+{FP\_y\_gapF\_starr}\, \left({{\tilde y^*}}_{t-1}-{{\tilde y^{cu}}}_{t-1}\right)+{FP\_pieF\_starr}\, \left({{\pi^{F*}}}_{t-1}-{{\pi^{cu}}}_{t-1}\right)
\end{dmath}
% Equation 92
\begin{dmath}
{{a}}_{t}={RHOA}\, {{a}}_{t-1}-{{\epsilon_a}}_{t}
\end{dmath}
% Equation 93
\begin{dmath}
{{a^*}}_{t}={RHOA}\, {{a^*}}_{t-1}-{{\epsilon_a^*}}_{t}
\end{dmath}
% Equation 94
\begin{dmath}
{a\_cu}_{t}={{a}}_{t}\, {{h}}+{{a^*}}_{t}\, \left(1-{{h}}\right)
\end{dmath}
